WIP

Phi_System/PhiSem/PhiSem_Machine_Integer_Lib.thy
@@ -1,8 +1,6 @@
-theory PhiSem_Min_Lib
-  imports PhiSem_Min
+theory PhiSem_Machine_Integer_Lib
+  imports PhiSem_Machine_Integer
 begin
-
-chapter \<open>Program Library for Minimal Semantics\<close>
 
 section \<open>Preliminary\<close>
 
@@ -15,147 +13,6 @@ abbreviation LshR (infixl "LSHR" 70) where \<open>x LSHR y \<equiv> x div 2 ^ Bi
 abbreviation LshL (infixl "LSHL" 70) where \<open>x LSHL y \<equiv> x  *  2 ^ Big y\<close>
 
 definition Bits_Tag :: \<open>'a \<Rightarrow> nat \<Rightarrow> 'a\<close> (infix "<bits>" 25) where [iff]: \<open>(x <bits> n) = x\<close>
-
-section \<open>Basic Operations\<close>
-
-subsection \<open>Variable\<close>
-
-subsubsection \<open>Syntax\<close>
-
-syntax "__var__" :: "idt \<Rightarrow> logic" ("\<^bold>v\<^bold>a\<^bold>r _" [1000] 999)
-
-parse_ast_translation \<open>
-  let open Ast
-    fun mk_Var name =
-      Appl [Constant \<^const_syntax>\<open>\<phi>Type\<close>, Constant \<^const_syntax>\<open>Pure.dummy_pattern\<close>,
-        Appl [Variable "Var", name, Constant \<^const_syntax>\<open>Pure.dummy_pattern\<close>]]
-   in [(\<^syntax_const>\<open>__var__\<close>, fn ctxt => fn [name] => mk_Var name)]
-  end
-\<close>
-
-syntax "__get_var__" :: "idt \<Rightarrow> logic" ("$_" [1000] 999)
-consts "get_var____\<phi>" :: "varname \<Rightarrow> 'b"
-
-translations "$x" => "CONST get_var____\<phi> x"
-
-definition Variable_of :: \<open>'a \<Rightarrow> varname \<Rightarrow> 'a\<close> (infix "<val-of-var>" 22)
-  where [iff]: \<open>(S <val-of-var> V) = S\<close>
-
-definition Set_Variable :: \<open>varname \<Rightarrow> 'a \<Rightarrow> 'a\<close> ("$_ := _" [1000, 51] 50)
-  where [iff]: \<open>($x := y) = y\<close>
-
-lemma [\<phi>reason 2000 for
-  \<open>Synthesis_Parse (?var::varname) (?Y::?'ret \<Rightarrow> assn)\<close>
-]:
-  \<open>Synthesis_Parse var (\<lambda>_. x \<Ztypecolon> Var var T :: assn)\<close>
-  unfolding Synthesis_Parse_def ..
-
-
-\<phi>processor get_variable 5000 (\<open>\<^bold>c\<^bold>u\<^bold>r\<^bold>r\<^bold>e\<^bold>n\<^bold>t ?blk [?H] \<^bold>r\<^bold>e\<^bold>s\<^bold>u\<^bold>l\<^bold>t\<^bold>s \<^bold>i\<^bold>n ?T\<close>)  \<open>
-  fn (ctxt,sequent) => \<^keyword>\<open>$\<close> |-- Parse.term >> (fn var => fn () =>
-    let
-      val ctxt_parse = Config.put phi_synthesis_parsing true ctxt
-      val term = Const(\<^const_name>\<open>get_var____\<phi>\<close>, dummyT) $ Syntax.parse_term ctxt_parse var
-                  |> Syntax.check_term ctxt_parse
-                  |> Thm.cterm_of ctxt
-    in
-      NuSys.synthesis term (ctxt,sequent)
-    end)
-\<close>
-
-
-subsubsection \<open>Operations\<close>
-
-paragraph \<open>Get Variable\<close>
-
-proc (nodef) op_get_var:
-  assumes [unfolded \<phi>SemType_def subset_iff, useful]: \<open>\<phi>SemType (x \<Ztypecolon> T) TY\<close>
-  argument \<open>x \<Ztypecolon> Var vname T\<close>
-  return   \<open>x \<Ztypecolon> Var vname T\<heavy_comma> \<^bold>v\<^bold>a\<^bold>l x \<Ztypecolon> T\<close>
-  \<medium_left_bracket> to_Identity op_get_var'' \<medium_right_bracket> using \<phi> by simp .
-
-lemma [\<phi>reason for \<open>\<^bold>p\<^bold>r\<^bold>o\<^bold>c ?f \<lbrace> ?R \<longmapsto> \<lambda>ret. ?R'\<heavy_comma> SYNTHESIS ?x <val-of-var> ?var \<Ztypecolon> ?T ret \<^bold>t\<^bold>h\<^bold>r\<^bold>o\<^bold>w\<^bold>s ?E \<rbrace> \<^bold>@\<^bold>G\<^bold>O\<^bold>A\<^bold>L ?G\<close>]:
-  \<open> SUBGOAL G G2
-\<Longrightarrow> \<^bold>v\<^bold>i\<^bold>e\<^bold>w X \<longmapsto> Y\<heavy_comma> \<blangle> x \<Ztypecolon> Var var T \<brangle> \<^bold><\<^bold>a\<^bold>c\<^bold>t\<^bold>i\<^bold>o\<^bold>n\<^bold>> ToSA \<^bold>@\<^bold>G\<^bold>O\<^bold>A\<^bold>L G2
-\<Longrightarrow> SOLVE_SUBGOAL G2
-\<Longrightarrow> \<phi>SemType (x \<Ztypecolon> T) TY
-\<Longrightarrow> \<^bold>p\<^bold>r\<^bold>o\<^bold>c op_get_var var TY \<lbrace> X \<longmapsto> Y\<heavy_comma> x \<Ztypecolon> Var var T \<heavy_comma> SYNTHESIS \<^bold>v\<^bold>a\<^bold>l x <val-of-var> var \<Ztypecolon> T \<rbrace> \<^bold>@\<^bold>G\<^bold>O\<^bold>A\<^bold>L G\<close>
-  unfolding Action_Tag_def
-  \<medium_left_bracket> premises _ and GetVar and _ and [\<phi>reason for \<open>\<phi>SemType (x \<Ztypecolon> T) ?TY\<close>]
-    GetVar op_get_var \<medium_right_bracket>. .
-
-
-
-paragraph \<open>Set Variable\<close>
-
-proc (nodef) op_set_var:
-  assumes [unfolded \<phi>SemType_def subset_iff, useful]: \<open>\<phi>SemType (x \<Ztypecolon> T) TY\<close>
-  assumes [unfolded \<phi>SemType_def subset_iff, useful]: \<open>\<phi>SemType (y \<Ztypecolon> U) TY\<close>
-  argument \<open>x \<Ztypecolon> Var var T\<heavy_comma> \<^bold>v\<^bold>a\<^bold>l y \<Ztypecolon> U\<close>
-  return   \<open>y \<Ztypecolon> Var var U\<close>
-  \<medium_left_bracket> to_Identity \<open>var\<close> to_Identity op_set_var'' \<medium_right_bracket>. .
-
-proc (nodef) op_set_var__synthesis[
-  \<phi>reason for \<open>\<^bold>p\<^bold>r\<^bold>o\<^bold>c ?f \<lbrace> ?R \<longmapsto> \<lambda>ret. ?R'\<heavy_comma> SYNTHESIS ($?var := ?y) \<Ztypecolon> ?U ret \<^bold>t\<^bold>h\<^bold>r\<^bold>o\<^bold>w\<^bold>s ?E \<rbrace> \<^bold>@\<^bold>G\<^bold>O\<^bold>A\<^bold>L ?G\<close>
-]:
-assumes G: \<open>\<^bold>p\<^bold>r\<^bold>o\<^bold>c g \<lbrace> X \<longmapsto> X1\<heavy_comma> SYNTHESIS \<^bold>v\<^bold>a\<^bold>l y \<Ztypecolon> U \<^bold>t\<^bold>h\<^bold>r\<^bold>o\<^bold>w\<^bold>s E\<rbrace> \<^bold>@\<^bold>G\<^bold>O\<^bold>A\<^bold>L G \<close>
-  and S[unfolded Action_Tag_def]:
-        \<open>\<And>vy. \<^bold>v\<^bold>i\<^bold>e\<^bold>w X1\<heavy_comma> y \<Ztypecolon> Val vy U \<longmapsto> Y\<heavy_comma> x \<Ztypecolon> Var var T\<heavy_comma> y \<Ztypecolon> Val vy U \<^bold>w\<^bold>i\<^bold>t\<^bold>h Any \<^bold><\<^bold>a\<^bold>c\<^bold>t\<^bold>i\<^bold>o\<^bold>n\<^bold>> ToSA\<close>
-  and [\<phi>reason for \<open>\<phi>SemType (x \<Ztypecolon> T) ?TY\<close>]: \<open>\<phi>SemType (x \<Ztypecolon> T) TY\<close>
-  and [\<phi>reason for \<open>\<phi>SemType (y \<Ztypecolon> U) ?TY\<close>]: \<open>\<phi>SemType (y \<Ztypecolon> U) TY\<close>
- goal G
-argument \<open>X\<close>
-return   \<open>Y\<heavy_comma> y \<Ztypecolon> Var var U \<heavy_comma> SYNTHESIS \<^bold>v\<^bold>a\<^bold>l ($var := y) \<Ztypecolon> U\<close>
-throws   E
-  \<medium_left_bracket> G S op_set_var op_get_var \<medium_right_bracket>. .
-
-
-paragraph \<open>Declare New Variables\<close>
-
-
-declare [[ML_print_depth=1000, eta_contract=false]]
-
-proc op_var_scope:
-  assumes [unfolded \<phi>SemType_def subset_iff, useful]: \<open>\<phi>SemType (x \<Ztypecolon> T) TY\<close>
-    and BLK: \<open>\<forall>var. \<^bold>p\<^bold>r\<^bold>o\<^bold>c F var \<lbrace> X\<heavy_comma> x \<Ztypecolon> Var var T \<longmapsto> \<lambda>ret. Y ret\<heavy_comma> () \<Ztypecolon> Var var (\<phi>Any <of-type> TY)
-                    \<^bold>t\<^bold>h\<^bold>r\<^bold>o\<^bold>w\<^bold>s \<lambda>v. E v \<heavy_comma> () \<Ztypecolon> Var var (\<phi>Any <of-type> TY) \<rbrace>\<close>
-  argument \<open>X\<heavy_comma> \<^bold>v\<^bold>a\<^bold>l x \<Ztypecolon> T\<close>
-  return   \<open>Y\<close>
-  throws   E
-  \<medium_left_bracket> to_Identity op_var_scope'
-    try'' \<medium_left_bracket> BLK to_Identity op_free_var \<medium_right_bracket>. \<medium_left_bracket> to_Identity op_free_var throw \<medium_right_bracket>. \<medium_right_bracket>. .
-
-lemma "__\<phi>op_var_scope__":
-  \<open> (\<And>var. \<^bold>p\<^bold>r\<^bold>o\<^bold>c F var \<lbrace> R\<heavy_comma> x \<Ztypecolon> Var var T\<heavy_comma>  X \<longmapsto> \<lambda>ret. Y ret \<heavy_comma> () \<Ztypecolon> Var var (\<phi>Any <of-type> TY)
-                \<^bold>t\<^bold>h\<^bold>r\<^bold>o\<^bold>w\<^bold>s \<lambda>v. E v \<heavy_comma> () \<Ztypecolon> Var var (\<phi>Any <of-type> TY) \<rbrace>)
-\<Longrightarrow> \<phi>SemType (x \<Ztypecolon> T) TY
-\<Longrightarrow> \<^bold>p\<^bold>r\<^bold>o\<^bold>c op_var_scope TYPE('a) TY F raw \<lbrace> R\<heavy_comma> (X\<heavy_comma> x \<Ztypecolon> Val raw T) \<longmapsto> \<lambda>ret. Y ret \<^bold>t\<^bold>h\<^bold>r\<^bold>o\<^bold>w\<^bold>s E \<rbrace>\<close>
-  unfolding mult.assoc[symmetric]
-  using op_var_scope_\<phi>app[where X=\<open>R\<heavy_comma> X\<close> and x = x and T = T and TY = TY and F=F,
-            of Y E \<open>raw\<close>, simplified]
-  by (smt (verit, best) ab_semigroup_mult_class.mult_ac(1) mult.commute)
-
-lemma "__\<phi>op_set_var__":
-  \<open> \<^bold>p\<^bold>r\<^bold>o\<^bold>c g \<lbrace> R\<heavy_comma> y \<Ztypecolon> Var var U\<heavy_comma> X \<longmapsto> Z \<^bold>t\<^bold>h\<^bold>r\<^bold>o\<^bold>w\<^bold>s E \<rbrace>
-\<Longrightarrow> \<phi>SemType (x \<Ztypecolon> T) TY
-\<Longrightarrow> \<phi>SemType (y \<Ztypecolon> U) TY
-\<Longrightarrow> \<^bold>p\<^bold>r\<^bold>o\<^bold>c (op_set_var var TY raw \<ggreater> g) \<lbrace> R\<heavy_comma> (X\<heavy_comma> x \<Ztypecolon> Var var T \<heavy_comma> y \<Ztypecolon> Val raw U) \<longmapsto> Z \<^bold>t\<^bold>h\<^bold>r\<^bold>o\<^bold>w\<^bold>s E \<rbrace>\<close>
-  \<medium_left_bracket> premises G and [\<phi>reason for \<open>\<phi>SemType (x \<Ztypecolon> T) ?TY\<close>] and [\<phi>reason for \<open>\<phi>SemType (y \<Ztypecolon> U) ?TY\<close>]
-    op_set_var G \<medium_right_bracket>. .
-
-
-lemma "__\<phi>op_var_scope__0":
-  \<open> \<^bold>p\<^bold>r\<^bold>o\<^bold>c F \<lbrace> R \<longmapsto> Y \<^bold>t\<^bold>h\<^bold>r\<^bold>o\<^bold>w\<^bold>s E \<rbrace>
-\<Longrightarrow> \<^bold>p\<^bold>r\<^bold>o\<^bold>c F \<lbrace> R\<heavy_comma> Void \<longmapsto> Y \<^bold>t\<^bold>h\<^bold>r\<^bold>o\<^bold>w\<^bold>s E \<rbrace>\<close>
-  by fastforce
-
-ML_file_debug "library/local_value.ML"
-
-\<phi>processor assign_variable 7500 (\<open>\<^bold>c\<^bold>u\<^bold>r\<^bold>r\<^bold>e\<^bold>n\<^bold>t ?blk [?H] \<^bold>r\<^bold>e\<^bold>s\<^bold>u\<^bold>l\<^bold>t\<^bold>s \<^bold>i\<^bold>n ?S\<close>) \<open>
-  fn (ctxt,sequent) => ((\<^keyword>\<open>\<rightarrow>\<close> |-- Parse.list1 Parse.binding)
->> (fn vars => fn () =>
-  raise NuProcessor.Terminate_Process (Local_Value.mk_var_scope vars (ctxt,sequent), I)))
-\<close>
 
 
 subsection \<open>Arithmetic Operations\<close>
@@ -222,7 +79,6 @@ proc [
   return   \<open>R2\<heavy_comma> SYNTHESIS \<^bold>v\<^bold>a\<^bold>l (x \<or> y) \<Ztypecolon> \<bool>\<close>
   throws \<open>E1 + E2\<close>
   \<medium_left_bracket> F1 F2 \<or> \<medium_right_bracket>. .
-
 
 subsubsection \<open>Constant Integer\<close>
 
@@ -310,14 +166,11 @@ proc [
   throws \<open>E1 + E2\<close>
   \<medium_left_bracket> F1 F2 + \<medium_right_bracket>. .
 
-
 lemma op_add_mod:
   \<open> \<^bold>p\<^bold>r\<^bold>o\<^bold>c op_add b (\<phi>V_pair vy vx) \<lbrace> x \<Ztypecolon> Val vx \<nat>[b]\<heavy_comma> y \<Ztypecolon> Val vy \<nat>[b] \<longmapsto> \<^bold>v\<^bold>a\<^bold>l (x + y) mod 2 ^ Big b \<Ztypecolon> \<nat>[b] \<rbrace>\<close>
   unfolding op_add_def including unfold_Big
   by (cases vx; cases vy; simp, rule, rule, simp add: \<phi>expns, rule,
       simp add: \<phi>expns, rule, simp add: \<phi>expns)
-
-
 
 paragraph \<open>Subtraction\<close>
 
@@ -362,7 +215,6 @@ proc [
   return   \<open>R2\<heavy_comma> SYNTHESIS \<^bold>v\<^bold>a\<^bold>l (x * y) \<Ztypecolon> \<nat>[b]\<close>
   throws \<open>E1 + E2\<close>
   \<medium_left_bracket> F1 F2 * \<medium_right_bracket>. .
-
 
 
 paragraph \<open>Division\<close>
@@ -479,6 +331,7 @@ proc [
   throws \<open>E1 + E2\<close>
   \<medium_left_bracket> F1 F2 \<le> \<medium_right_bracket>. .
 
+
 proc [
     \<phi>reason for \<open>\<^bold>p\<^bold>r\<^bold>o\<^bold>c ?F \<lbrace> ?R \<longmapsto> \<lambda>ret. ?R2\<heavy_comma> SYNTHESIS (?x \<ge> ?y) \<Ztypecolon> ?T ret \<^bold>t\<^bold>h\<^bold>r\<^bold>o\<^bold>w\<^bold>s ?E \<rbrace> \<^bold>@\<^bold>G\<^bold>O\<^bold>A\<^bold>L ?G\<close>
 ]:
@@ -524,8 +377,6 @@ proc \<phi>__synthesis_eq[
   return   \<open>R2\<heavy_comma> SYNTHESIS \<^bold>v\<^bold>a\<^bold>l (x = y) \<Ztypecolon> \<bool>\<close>
   throws \<open>E1 + E2\<close>
   \<medium_left_bracket> F1 F2 = \<medium_right_bracket>. .
-
-
 
 subsection \<open>Branches & Loops\<close>
 
@@ -645,42 +496,5 @@ proc while:
   \<medium_right_bracket>. .
 
 
-(*Example*)
-
-
-proc AA:
-  argument \<open>\<^bold>v\<^bold>a\<^bold>l 1 \<Ztypecolon> \<nat>[32]\<heavy_comma> \<^bold>v\<^bold>a\<^bold>l 2 \<Ztypecolon> \<nat>[32]\<heavy_comma> \<^bold>v\<^bold>a\<^bold>l 3 \<Ztypecolon> \<nat>[32]\<close>
-  return \<open>\<^bold>v\<^bold>a\<^bold>l 6 \<Ztypecolon> \<nat>[32]\<heavy_comma> \<^bold>v\<^bold>a\<^bold>l 4 \<Ztypecolon> \<nat>[32]\<heavy_comma> \<^bold>v\<^bold>a\<^bold>l 2 \<Ztypecolon> \<nat>[32]\<close>
-  \<medium_left_bracket> + + 4 2 1 - 1 + 30000 * 30000 /  \<medium_right_bracket>. .
-
-thm op_const_int_\<phi>app
-thm AA_\<phi>compilation
-
-(*
-int XX(int x) { if 0 < x then x - 1 else 0 }
-*)
-proc
-  argument \<open>\<^bold>v\<^bold>a\<^bold>l x \<Ztypecolon> \<nat>[32]\<close>
-  return \<open>\<^bold>v\<^bold>a\<^bold>l x - 1 \<Ztypecolon> \<nat>[32]\<close>
-  \<medium_left_bracket> \<rightarrow> varx
-  ;; (*assign the value x to a variable named varx*)
-     (* command `;;` leads a statement, or ends the previous statement. *)
-    if \<medium_left_bracket> \<open>0 < $varx\<close> \<medium_right_bracket>. \<medium_left_bracket> \<open>$varx - 1\<close> \<medium_right_bracket>. \<medium_left_bracket> \<open>0::nat\<close> \<medium_right_bracket>.
-    (* the cartouche like \<open>0 < $varx\<close> invokes a synthesis process
-       to make that value automatically *)
-  \<medium_right_bracket> using \<phi> by simp .
-
-
-
-proc
-  premises \<open>x < 10\<close>
-  argument \<open>\<^bold>v\<^bold>a\<^bold>l x \<Ztypecolon> \<nat>[32]\<close>
-  return \<open>\<^bold>v\<^bold>a\<^bold>l 10 \<Ztypecolon> \<nat>[32]\<close>
-  \<medium_left_bracket> \<rightarrow> v ;;
-    while \<open>xxx \<Ztypecolon> ?X \<^bold>s\<^bold>u\<^bold>b\<^bold>j xxx. Inv: (xxx \<le> 10) \<and> Guard: xxx < 10\<close> (*specification*)
-    \<medium_left_bracket> \<open>$v < 10\<close> \<medium_right_bracket>. (*guard*)
-    \<medium_left_bracket> \<open>$v + 1\<close> \<rightarrow> v \<medium_right_bracket>. (*loop body*)
-    $v
-  \<medium_right_bracket>. .
 
 end
