Phi_System/PhiSem/PhiSem_Generic_Boolean.thy
@@ -1,0 +1,10 @@
+theory PhiSem_Generic_Boolean
+  imports Phi_System.PhiSem_Formalization_Tools
+begin
+
+section \<open>\<close>
+
+consts bool :: TY
+
+
+end
