Phi_System/PhiSem/PhiSem_Machine_Integer.thy
@@ -1,0 +1,386 @@
+theory PhiSem_Machine_Integer
+  imports Phi_System.PhiSem_Formalization_Tools
+begin
+
+chapter \<open>Semantics for Machine Integers\<close>
+
+section \<open>Preliminary\<close>
+
+no_notation inter (infixl "Int" 70) and union (infixl "Un" 65)
+
+subsection \<open>Models\<close>
+
+subsubsection \<open>Type\<close>
+
+virtual_datatype \<phi>min_ty = \<phi>empty_ty +
+  T_int     :: nat \<comment> \<open>in unit of bits\<close>
+
+context \<phi>min_ty begin
+abbreviation int where \<open>int \<equiv> T_int.mk\<close>
+end
+
+debt_axiomatization T_int :: \<open>nat type_entry\<close>
+  where \<phi>min_ty_ax: \<open>\<phi>min_ty TY_CONS_OF T_int\<close>
+
+interpretation \<phi>min_ty TY_CONS_OF _ _ T_int using \<phi>min_ty_ax .
+
+hide_fact \<phi>min_ty_ax \<phi>min_ty_axioms \<phi>min_ty_names_def \<phi>min_ty_def
+  \<phi>min_ty_prjs_axioms \<phi>min_ty_prjs_def \<phi>min_ty.axioms \<phi>min_ty.intro
+  \<phi>min_ty__names.\<phi>min_ty_names_axioms \<phi>min_ty_prjs.axioms
+
+subsubsection \<open>Value\<close>
+
+virtual_datatype \<phi>min_val = \<phi>empty_val +
+  V_int     :: \<open>nat \<times> nat\<close> \<comment> \<open>bits \<times> value\<close>
+
+debt_axiomatization V_int :: \<open>(nat \<times> nat) value_entry\<close>
+  where \<phi>min_val_ax: \<open>\<phi>min_val VAL_CONS_OF V_int\<close>
+
+interpretation \<phi>min_val VAL_CONS_OF _ _ V_int using \<phi>min_val_ax .
+
+hide_fact \<phi>min_val_ax \<phi>min_val_axioms
+
+subsubsection \<open>Semantics\<close>
+
+debt_axiomatization
+    WT_int[simp]: \<open>Well_Type (int b)     = { V_int.mk (b,x)    |x. x < 2 ^ Big b } \<close>
+and can_eqcmp_int[simp]: "Can_EqCompare res (V_int.mk (b1,x1)) (V_int.mk (b2,x2)) \<longleftrightarrow> b1 = b2"
+and eqcmp_int[simp]: "EqCompare (V_int.mk i1) (V_int.mk i2) \<longleftrightarrow> i1 = i2"
+and  zero_int[simp]: \<open>Zero (int b)    = Some (V_int.mk (b,0))\<close>
+
+lemma Valid_Types[simp]:
+  \<open>Valid_Type (int n)\<close>
+  unfolding Inhabited_def
+  apply simp
+  using less_exp by blast
+
+
+section \<open>\<phi>-Types\<close>
+
+\<phi>overloads nat and int
+
+subsection \<open>Integer\<close>
+
+subsubsection \<open>Natural Nmbers\<close>
+
+paragraph \<open>Natural Number\<close>
+
+definition \<phi>Nat :: "nat \<Rightarrow> (VAL, nat) \<phi>" ("\<nat>[_]")
+  where "\<nat>[b] x = (if x < 2^b then { V_int.mk (b,x) } else {})"
+
+lemma \<phi>Nat_expn[\<phi>expns]:
+  "p \<in> (x \<Ztypecolon> \<nat>[b]) \<longleftrightarrow> (p = V_int.mk (b,x)) \<and> x < 2 ^ Big b"
+  unfolding \<phi>Type_def Big_def by (simp add: \<phi>Nat_def)
+
+lemma \<phi>Nat_elim[elim!,\<phi>inhabitance_rule]:
+  "Inhabited (x \<Ztypecolon> \<nat>[b]) \<Longrightarrow> (x < 2 ^ Big b \<Longrightarrow> C) \<Longrightarrow> C"
+  unfolding Inhabited_def by (simp add: \<phi>expns)
+
+lemma \<open>Inhabited (x \<Ztypecolon> \<nat>[b]) \<longleftrightarrow> x < 2^Big b\<close>
+  unfolding Inhabited_def by (simp add: \<phi>expns)
+
+lemma \<phi>Nat_semty[\<phi>reason for \<open>\<phi>SemType (?x \<Ztypecolon> \<nat>[?b]) ?ty\<close>]:
+  \<open>\<phi>SemType (x \<Ztypecolon> \<nat>[b]) (int b)\<close>
+  unfolding \<phi>SemType_def subset_iff by (simp add: \<phi>expns Big_def)
+
+lemma [\<phi>reason for \<open>\<phi>Equal (\<nat>[?b]) ?c ?eq\<close>]:
+  "\<phi>Equal (\<nat>[b]) (\<lambda>x y. True) (=)"
+  unfolding \<phi>Equal_def by (auto simp add: \<phi>expns)
+
+lemma [\<phi>reason for \<open>\<phi>Zero (int ?b) (\<nat>[?b]) ?zero\<close>]:
+  "\<phi>Zero (int b) (\<nat>[b]) 0" unfolding \<phi>Zero_def by (simp add: \<phi>expns)
+
+lemma [\<phi>reason]:
+  \<open> \<^bold>p\<^bold>r\<^bold>e\<^bold>m\<^bold>i\<^bold>s\<^bold>e x < 2^Big b
+\<Longrightarrow> is_singleton (x \<Ztypecolon> \<nat>[b])\<close>
+  by (rule is_singletonI''; simp add: \<phi>expns)
+
+paragraph \<open>Rounded Natural Number\<close>
+
+definition \<phi>NatRound :: "nat \<Rightarrow> (VAL, nat) \<phi>" ("\<nat>\<^sup>r[_]")
+  where "\<nat>\<^sup>r[b] x = { V_int.mk (b, (x mod 2 ^ Big b)) }"
+
+lemma \<phi>NatRound_expn[\<phi>expns]:
+  "p \<in> (x \<Ztypecolon> \<nat>\<^sup>r[b]) \<longleftrightarrow> p = V_int.mk (b, (x mod 2 ^ Big b))"
+  unfolding \<phi>Type_def \<phi>NatRound_def by simp
+
+lemma \<open>Inhabited (x \<Ztypecolon> \<nat>\<^sup>r[b]) \<longleftrightarrow> True\<close>
+  unfolding Inhabited_def by (auto simp add: \<phi>expns)
+
+lemma [\<phi>reason for \<open>\<phi>Zero (int ?b) \<nat>\<^sup>r[?b] ?z\<close>]:
+  "\<phi>Zero (int b) (\<nat>\<^sup>r[b]) 0"
+  unfolding \<phi>Zero_def by (simp add: \<phi>expns)
+
+lemma \<phi>NatRound_semty[\<phi>reason for \<open>\<phi>SemType (?x \<Ztypecolon> \<nat>\<^sup>r[?b]) ?ty\<close>]:
+  \<open>\<phi>SemType (x \<Ztypecolon> \<nat>\<^sup>r[b]) (int b)\<close>
+  unfolding \<phi>SemType_def subset_iff by (simp add: \<phi>expns)
+
+
+subsubsection \<open>Integer in the normal sense\<close>
+
+definition \<phi>Int :: "nat \<Rightarrow> (VAL, int) \<phi>" ("\<int>[_]")
+  where "\<phi>Int b x =(if x < 2^(b - 1) \<and> -(2^(b-1)) \<le> x \<and> (b = 0 \<longrightarrow> x = 0)
+                    then { V_int.mk (b, (if x \<ge> 0 then nat x else nat (2^b + x))) }
+                    else {})"
+
+lemma \<phi>Int_expn[\<phi>expns]:
+  "p \<in> (x \<Ztypecolon> \<int>[b]) \<longleftrightarrow> p = V_int.mk (b, (if x \<ge> 0 then nat x else nat (2^b + x)))
+                      \<and> x < 2^(b - 1) \<and> -(2^(b-1)) \<le> x \<and> (b = 0 \<longrightarrow> x = 0)"
+  unfolding \<phi>Type_def by (simp add: \<phi>Int_def)
+
+lemma \<phi>Int_inhabited[elim!,\<phi>inhabitance_rule]:
+  "Inhabited (x \<Ztypecolon> \<int>[b]) \<Longrightarrow> (x < 2^(b - 1) \<and> -(2^(b-1)) \<le> x \<and> (b = 0 \<longrightarrow> x = 0) \<Longrightarrow> C) \<Longrightarrow> C"
+  unfolding Inhabited_def by (simp add: \<phi>expns) 
+
+lemma [simp]: \<open>- (2^(b - 1)) \<le> x \<Longrightarrow> 0 \<le> 2 ^ b + x\<close> for x :: int
+  by (smt (verit, best) diff_le_self power_increasing_iff)
+
+lemma [\<phi>reason for \<open>\<phi>Equal \<int>[b] ?c ?eq\<close>]:
+    "\<phi>Equal \<int>[b] (\<lambda>x y. True) (=)"
+  unfolding \<phi>Equal_def by (cases b) (auto simp add: \<phi>expns eq_nat_nat_iff)
+
+lemma [\<phi>reason for \<open>\<phi>Zero (int ?b) \<int>[?b] ?x\<close>]:
+    "\<phi>Zero (int b) \<int>[b] 0"
+  unfolding \<phi>Zero_def by (simp add: \<phi>expns)
+
+
+lemma \<phi>Int_semty[\<phi>reason for \<open>\<phi>SemType (?x \<Ztypecolon> \<int>[?b]) ?ty\<close>]:
+  \<open>\<phi>SemType (x \<Ztypecolon> \<int>[b]) (int b)\<close>
+  unfolding \<phi>SemType_def subset_iff
+  by (simp add: \<phi>expns Big_def) (smt (verit, ccfv_SIG) diff_le_self power_increasing_iff)
+
+
+subsubsection \<open>Subtyping\<close>
+
+lemma subty_Z_N[\<phi>overload nat]: 
+  "\<^bold>p\<^bold>r\<^bold>e\<^bold>m\<^bold>i\<^bold>s\<^bold>e 0 < x \<Longrightarrow> x \<Ztypecolon> \<int>[b] \<^bold>i\<^bold>m\<^bold>p\<^bold>l\<^bold>i\<^bold>e\<^bold>s nat x \<Ztypecolon> \<nat>[b]"
+  unfolding Imply_def Premise_def apply (simp add: \<phi>expns Big_def del: One_nat_def)
+  by (smt (verit, del_insts) diff_less less_numeral_extra(1) power_strict_increasing_iff)
+
+lemma subty_N_Z[\<phi>overload int]:
+  "\<^bold>p\<^bold>r\<^bold>e\<^bold>m\<^bold>i\<^bold>s\<^bold>e x < 2^(b - 1) \<Longrightarrow> x \<Ztypecolon> \<nat>[b] \<^bold>i\<^bold>m\<^bold>p\<^bold>l\<^bold>i\<^bold>e\<^bold>s Int.int x \<Ztypecolon> \<int>[b]"
+  unfolding Imply_def Premise_def apply (simp add: \<phi>expns Big_def del: One_nat_def)
+  by (metis less_one linorder_le_cases neg_0_le_iff_le not_exp_less_eq_0_int of_nat_0_le_iff order_trans power_0)
+
+
+subsubsection \<open>Boolean\<close>
+
+(* lemma [simp]: "(x \<noteq> 1) = (x = 0)" for x :: "1 word" proof -
+  have "(UNIV:: 1 word set) = {0,1}" unfolding UNIV_word_eq_word_of_nat
+  using less_2_cases apply auto apply force
+  by (metis UNIV_I UNIV_word_eq_word_of_nat len_num1 power_one_right)
+  then show ?thesis  by auto
+qed *)
+
+definition \<phi>Bool :: "(VAL, bool) \<phi>" ("\<bool>")
+  where "\<bool> x = { V_int.mk (1, (if x then 1 else 0)) }"
+
+lemma \<phi>Bool_expn[\<phi>expns]:
+  " p \<in> (x \<Ztypecolon> \<bool>) \<longleftrightarrow> p = V_int.mk (1, (if x then 1 else 0))"
+  unfolding \<phi>Type_def \<phi>Bool_def by simp
+
+lemma \<phi>Bool_inhabited[\<phi>inhabitance_rule, elim!]:
+  \<open>Inhabited (x \<Ztypecolon> \<bool>) \<Longrightarrow> C \<Longrightarrow> C\<close> .
+
+lemma \<phi>Bool_eqcmp[\<phi>reason for \<open>\<phi>Equal \<bool> ?c ?eq\<close>]:
+  "\<phi>Equal \<bool> (\<lambda>x y. True) (=)"
+  unfolding \<phi>Equal_def by (simp add: \<phi>expns)
+
+lemma \<phi>Bool_zero[\<phi>reason for \<open>\<phi>Zero (int 1) \<bool> ?z\<close>]:
+  "\<phi>Zero (int 1) \<bool> False"
+  unfolding \<phi>Zero_def by (simp add: \<phi>expns)
+
+lemma \<phi>Bool_semty[\<phi>reason for \<open>\<phi>SemType (?x \<Ztypecolon> \<bool>) ?ty\<close>]:
+  \<open>\<phi>SemType (x \<Ztypecolon> \<bool>) (int 1)\<close>
+  unfolding \<phi>SemType_def subset_iff
+  by (simp add: \<phi>expns Big_def)
+
+lemma [\<phi>reason]:
+  \<open>is_singleton (x \<Ztypecolon> \<bool>)\<close>
+  by (rule is_singletonI''; simp add: \<phi>expns)
+
+abbreviation \<open>Predicate_About x \<equiv> (\<bool> <func-over> x)\<close>
+
+
+section \<open>Instructions\<close>
+
+subsection \<open>Arithmetic Operations\<close>
+
+subsubsection \<open>Integer arithmetic\<close>
+
+definition op_const_int :: "nat \<Rightarrow> nat \<Rightarrow> VAL proc"
+  where "op_const_int bits const = Return (sem_value (V_int.mk (bits,const)))"
+
+(* definition op_const_size_t :: "nat \<Rightarrow> (VAL,VAL,'RES_N,'RES) proc"
+  where "op_const_size_t c = \<phi>M_assume (c < 2 ^ addrspace_bits)
+                          \<ggreater> Return (sem_value (V_int.mk (addrspace_bits,c)))"
+  \<comment> \<open> `op_const_size_t` checks the overflow during the compilation towards certain decided platform.  \<close>
+*)
+
+definition op_add :: "nat \<Rightarrow> (VAL \<times> VAL, VAL) proc'"
+  where "op_add bits =
+      \<phi>M_caseV (\<lambda>vb va.
+      \<phi>M_getV (int bits) (snd o V_int.dest) vb (\<lambda>val_b.
+      \<phi>M_getV (int bits) (snd o V_int.dest) va (\<lambda>val_a.
+      Return (sem_value (V_int.mk (bits, ((val_a + val_b) mod 2^bits))))
+  )))"
+
+definition op_sub :: "nat \<Rightarrow> (VAL \<times> VAL, VAL) proc'"
+  where "op_sub bits =
+      \<phi>M_caseV (\<lambda>va vb.
+      \<phi>M_getV (int bits) (snd o V_int.dest) va (\<lambda>val_a.
+      \<phi>M_getV (int bits) (snd o V_int.dest) vb (\<lambda>val_b.
+      Return (sem_value (V_int.mk (bits, ((2^bits + val_b - val_a) mod 2^bits))))
+  )))"
+
+definition op_umul :: "nat \<Rightarrow> (VAL \<times> VAL, VAL) proc'"
+  where "op_umul bits =
+      \<phi>M_caseV (\<lambda>va vb.
+      \<phi>M_getV (int bits) (snd o V_int.dest) va (\<lambda>val_a.
+      \<phi>M_getV (int bits) (snd o V_int.dest) vb (\<lambda>val_b.
+      Return (sem_value (V_int.mk (bits, ((val_b * val_a) mod 2^bits))))
+  )))"
+
+definition op_udiv :: "nat \<Rightarrow> (VAL \<times> VAL, VAL) proc'"
+  where "op_udiv bits =
+      \<phi>M_caseV (\<lambda>va vb.
+      \<phi>M_getV (int bits) (snd o V_int.dest) va (\<lambda>val_a.
+      \<phi>M_getV (int bits) (snd o V_int.dest) vb (\<lambda>val_b.
+      Return (sem_value (V_int.mk (bits, (val_b div val_a))))
+  )))"
+
+definition op_lshr :: "nat \<Rightarrow> nat \<Rightarrow> (VAL \<times> VAL, VAL) proc'"
+  where "op_lshr b_b b_a =
+      \<phi>M_caseV (\<lambda>va vb.
+      \<phi>M_getV (int b_a) (snd o V_int.dest) va (\<lambda>val_a.
+      \<phi>M_getV (int b_b) (snd o V_int.dest) vb (\<lambda>val_b.
+      Return (sem_value (V_int.mk (b_b, (val_b div 2 ^ val_a))))
+  )))"
+
+definition op_lshl :: "nat \<Rightarrow> nat \<Rightarrow> (VAL \<times> VAL, VAL) proc'"
+  where "op_lshl b_b b_a =
+      \<phi>M_caseV (\<lambda>va vb.
+      \<phi>M_getV (int b_a) (snd o V_int.dest) va (\<lambda>val_a.
+      \<phi>M_getV (int b_b) (snd o V_int.dest) vb (\<lambda>val_b.
+      Return (sem_value (V_int.mk (b_b, (val_b * 2 ^ val_a))))
+  )))"
+
+definition op_lt :: "nat \<Rightarrow> (VAL \<times> VAL, VAL) proc'"
+  where "op_lt bits =
+      \<phi>M_caseV (\<lambda>va vb.
+      \<phi>M_getV (int bits) (snd o V_int.dest) va (\<lambda>val_a.
+      \<phi>M_getV (int bits) (snd o V_int.dest) vb (\<lambda>val_b.
+      Return (sem_value (V_int.mk (1, (if val_b < val_a then 1 else 0))))
+  )))"
+
+definition op_le :: "nat \<Rightarrow> (VAL \<times> VAL, VAL) proc'"
+  where "op_le bits =
+      \<phi>M_caseV (\<lambda>va vb.
+      \<phi>M_getV (int bits) (snd o V_int.dest) va (\<lambda>val_a.
+      \<phi>M_getV (int bits) (snd o V_int.dest) vb (\<lambda>val_b.
+      Return (sem_value (V_int.mk (1, (if val_b \<le> val_a then 1 else 0))))
+  )))"
+
+
+definition op_not :: "(VAL, VAL) proc'"
+  where "op_not v =
+    \<phi>M_getV (int 1) (snd o V_int.dest) v (\<lambda>v.
+    Return (sem_value (V_int.mk (1, 1 - v)))
+  )"
+
+definition op_and :: "(VAL \<times> VAL, VAL) proc'"
+  where "op_and =
+    \<phi>M_caseV (\<lambda>va vb.
+    \<phi>M_getV (int 1) (snd o V_int.dest) va (\<lambda>v.
+    \<phi>M_getV (int 1) (snd o V_int.dest) vb (\<lambda>u.
+    Return (sem_value (V_int.mk (1, v+u-1)))
+  )))"
+
+definition op_or :: "(VAL \<times> VAL, VAL) proc'"
+  where "op_or =
+    \<phi>M_caseV (\<lambda>va vb.
+    \<phi>M_getV (int 1) (snd o V_int.dest) va (\<lambda>v.
+    \<phi>M_getV (int 1) (snd o V_int.dest) vb (\<lambda>u.
+    Return (sem_value (V_int.mk (1, min 1 (v+u))))
+  )))"
+
+definition op_equal :: "TY \<Rightarrow> (VAL \<times> VAL, VAL) proc'"
+  where "op_equal TY =
+    \<phi>M_caseV (\<lambda>va vb.
+    \<phi>M_getV TY id va (\<lambda>v.
+    \<phi>M_getV TY id vb (\<lambda>u.
+    (\<lambda>res. \<phi>M_assert (Can_EqCompare res u v) res) \<ggreater>
+    Return (sem_value (V_int.mk (1, (if EqCompare u v then 1 else 0))))
+)))"
+
+
+subsection \<open>Branches & Loops\<close>
+
+paragraph \<open>Non-Branching Selection\<close>
+
+definition op_sel :: "TY \<Rightarrow> (VAL \<times> VAL \<times> VAL, VAL) proc'"
+  where "op_sel TY =
+    \<phi>M_caseV (\<lambda>vc. \<phi>M_caseV (\<lambda>va vb.
+    \<phi>M_getV (int 1) V_int.dest vc (\<lambda>c.
+    \<phi>M_getV TY id va (\<lambda>a.
+    \<phi>M_getV TY id vb (\<lambda>b.
+    Return (sem_value (if snd c = 1 then b else a)))))))"
+
+paragraph \<open>Branch\<close>
+
+definition op_if :: "'ret proc
+                  \<Rightarrow> 'ret proc
+                  \<Rightarrow> (VAL,'ret) proc'"
+  where "op_if brT brF v =
+    \<phi>M_getV (int 1) V_int.dest v (\<lambda>c. (if snd c = 1 then brT else brF))"
+
+paragraph \<open>While Loop\<close>
+
+inductive SemDoWhile :: "VAL proc \<Rightarrow> resource \<Rightarrow> unit state \<Rightarrow> bool" where
+  "Success (sem_value (V_int.mk (1,0))) res \<in> f s \<Longrightarrow> SemDoWhile f s (Success (sem_value ()) res)"
+| "Success (sem_value (V_int.mk (1,1))) res \<in> f s \<Longrightarrow> SemDoWhile f res s'' \<Longrightarrow> SemDoWhile f s s''"
+| "Exception v e \<in> f s \<Longrightarrow> SemDoWhile f s (Exception v e)"
+| "PartialCorrect \<in> f s \<Longrightarrow> SemDoWhile f s PartialCorrect"
+| "Invalid \<in> f s \<Longrightarrow> SemDoWhile f s Invalid"
+
+lemma "\<nexists> y. SemDoWhile ((\<lambda>res. Return (sem_value (V_int.mk (1,1))) res) :: VAL proc) res y"
+  apply rule apply (elim exE) subgoal for y
+    apply (induct "((\<lambda>res. Return (sem_value (V_int.mk (1,1))) (res::resource)) :: VAL proc)" res y
+           rule: SemDoWhile.induct)
+       apply (simp_all add: Return_def det_lift_def) . .
+
+definition op_do_while :: " VAL proc \<Rightarrow> unit proc"
+  where "op_do_while f s = Collect (SemDoWhile f s)"
+
+(* lemma SemDoWhile_deterministic:
+  assumes "SemDoWhile c s s1"
+      and "SemDoWhile c s s2"
+    shows "s1 = s2"
+proof -
+  have "SemDoWhile c s s1 \<Longrightarrow> (\<forall>s2. SemDoWhile c s s2 \<longrightarrow> s1 = s2)"
+    apply (induct rule: SemDoWhile.induct)
+    by (subst SemDoWhile.simps, simp)+
+  thus ?thesis
+    using assms by simp
+qed
+
+lemma SemDoWhile_deterministic2:
+    "SemDoWhile body s x \<Longrightarrow> The ( SemDoWhile body s) = x"
+  using SemDoWhile_deterministic by blast *)
+
+
+paragraph \<open>Recursion\<close>
+
+inductive SemRec :: "(('a,'a) proc' \<Rightarrow> ('a,'a) proc')
+            \<Rightarrow> 'a sem_value \<Rightarrow> resource \<Rightarrow> 'a state set \<Rightarrow> bool"
+where
+  SemRec_I0: "(\<And>g. F g x res = y) \<Longrightarrow> SemRec F x res y"
+| SemRec_IS: "SemRec (F o F) x res y \<Longrightarrow> SemRec F x res y"
+
+definition op_recursion :: "TY list \<Rightarrow> TY list
+                         \<Rightarrow> (('a,'a) proc' \<Rightarrow> ('a,'a) proc')
+                         \<Rightarrow> ('a,'a) proc'"
+  where "op_recursion _ _ F x s = (if (\<exists>t. SemRec F x s t) then The (SemRec F x s) else {})"
+
+
+end
