Phi_System/PhiSem/PhiSem_Play_Ground.thy
@@ -1,0 +1,44 @@
+theory PhiSem_Play_Ground
+  imports PhiSem_Machine_Integer_Lib
+    PhiSem_Variable_Lib
+begin
+
+(*Example*)
+
+
+proc AA:
+  argument \<open>\<^bold>v\<^bold>a\<^bold>l 1 \<Ztypecolon> \<nat>[32]\<heavy_comma> \<^bold>v\<^bold>a\<^bold>l 2 \<Ztypecolon> \<nat>[32]\<heavy_comma> \<^bold>v\<^bold>a\<^bold>l 3 \<Ztypecolon> \<nat>[32]\<close>
+  return \<open>\<^bold>v\<^bold>a\<^bold>l 6 \<Ztypecolon> \<nat>[32]\<heavy_comma> \<^bold>v\<^bold>a\<^bold>l 4 \<Ztypecolon> \<nat>[32]\<heavy_comma> \<^bold>v\<^bold>a\<^bold>l 2 \<Ztypecolon> \<nat>[32]\<close>
+  \<medium_left_bracket> + + 4 2 1 - 1 + 30000 * 30000 /  \<medium_right_bracket>. .
+
+thm op_const_int_\<phi>app
+thm AA_\<phi>compilation
+
+(*
+int XX(int x) { if 0 < x then x - 1 else 0 }
+*)
+proc
+  argument \<open>\<^bold>v\<^bold>a\<^bold>l x \<Ztypecolon> \<nat>[32]\<close>
+  return \<open>\<^bold>v\<^bold>a\<^bold>l x - 1 \<Ztypecolon> \<nat>[32]\<close>
+  \<medium_left_bracket> \<rightarrow> varx
+  ;; (*assign the value x to a variable named varx*)
+     (* command `;;` leads a statement, or ends the previous statement. *)
+    if \<medium_left_bracket> \<open>0 < $varx\<close> \<medium_right_bracket>. \<medium_left_bracket> \<open>$varx - 1\<close> \<medium_right_bracket>. \<medium_left_bracket> \<open>0::nat\<close> \<medium_right_bracket>.
+    (* the cartouche like \<open>0 < $varx\<close> invokes a synthesis process
+       to make that value automatically *)
+  \<medium_right_bracket> using \<phi> by simp .
+
+
+proc
+  premises \<open>x < 10\<close>
+  argument \<open>\<^bold>v\<^bold>a\<^bold>l x \<Ztypecolon> \<nat>[32]\<close>
+  return \<open>\<^bold>v\<^bold>a\<^bold>l 10 \<Ztypecolon> \<nat>[32]\<close>
+  \<medium_left_bracket> \<rightarrow> v ;;
+    while \<open>xxx \<Ztypecolon> ?X \<^bold>s\<^bold>u\<^bold>b\<^bold>j xxx. Inv: (xxx \<le> 10) \<and> Guard: xxx < 10\<close> (*specification*)
+    \<medium_left_bracket> \<open>$v < 10\<close> \<medium_right_bracket>. (*guard*)
+    \<medium_left_bracket> \<open>$v + 1\<close> \<rightarrow> v \<medium_right_bracket>. (*loop body*)
+    $v
+  \<medium_right_bracket>. .
+
+
+end
