Phi_System/PhiTypes.thy
@@ -1457,8 +1457,8 @@ text \<open>\<phi>MayInit T relates a value with T if the value is initialized; 
 definition \<phi>MayInit :: \<open>TY \<Rightarrow> (VAL, 'x) \<phi> \<Rightarrow> (VAL uninit, 'x) \<phi>\<close>
   where \<open>\<phi>MayInit TY T x = ({uninitialized} \<^bold>s\<^bold>u\<^bold>b\<^bold>j (\<exists>z. Zero TY = Some z \<and> z \<in> (x \<Ztypecolon> T))) + initialized ` (x \<Ztypecolon> T <of-type> TY)\<close>
 
-abbreviation \<phi>Share_Some_Init ("\<fish_eye>\<lbrakk>_\<rbrakk> _" [0, 91] 90)
-  where \<open>\<phi>Share_Some_Init TY T \<equiv> \<fish_eye> \<phi>MayInit TY T\<close>
+(* abbreviation \<phi>Share_Some_Init ("\<fish_eye>\<lbrakk>_\<rbrakk> _" [0, 91] 90)
+  where \<open>\<phi>Share_Some_Init TY T \<equiv> \<fish_eye> \<phi>MayInit TY T\<close> *)
 
 lemma \<phi>MayInit_expn[\<phi>expns]:
   \<open>p \<in> (x \<Ztypecolon> \<phi>MayInit TY T) \<longleftrightarrow> (p = uninitialized \<and> (\<exists>z. Zero TY = Some z \<and> z \<in> (x \<Ztypecolon> T)) \<or> (\<exists>v. p = initialized v \<and> v \<in> (x \<Ztypecolon> T <of-type> TY)))\<close>
